theories/Cargo.v
@@ -2646,19 +2646,19 @@ Module Cargo (N V F G CfgS Src : UsualOrderedType) (PM : SemverMatch V).
                             | reflexivity].
     Qed.
 
-    Lemma linkRel_headFibre : forall g Links l,
-        linkRel g (LinkFibred.headFibre Links l) =
+    Lemma linkRel_withHead : forall g Links l,
+        linkRel g (LinkFibred.withHead Links l) =
         ClsT.Reduction.Lookup.classRelAt (linkRel g Links) (NPlus.CLink l).
     Proof.
       intros; apply ClsT.InClassRel.ext; intros [q k].
       rewrite ClsT.Reduction.Lookup.mem_classRelAt, !mem_linkRel.
       split.
       - intros [m [v [l' [Hl [-> ->]]]]].
-        apply LinkFibred.mem_headFibre in Hl; destruct Hl as [Hl ->].
+        apply LinkFibred.mem_withHead in Hl; destruct Hl as [Hl ->].
         split; [exists m, v, l; repeat split; exact Hl | reflexivity].
       - intros [[m [v [l' [Hl [-> ->]]]]] Ek]; injection Ek as ->.
         exists m, v, l; repeat split.
-        apply LinkFibred.mem_headFibre; split; [exact Hl | reflexivity].
+        apply LinkFibred.mem_withHead; split; [exact Hl | reflexivity].
     Qed.
 
     Theorem versions_lookupLink :
@@ -2666,14 +2666,14 @@ Module Cargo (N V F G CfgS Src : UsualOrderedType) (PM : SemverMatch V).
         versions I (NPlus.CLink l) =
         versions
           (MkInst (claimants (inst_repo I) (inst_links I) l) SupportSet.empty
-             FDefRel.empty SlotRel.empty (LinkFibred.headFibre (inst_links I) l)
+             FDefRel.empty SlotRel.empty (LinkFibred.withHead (inst_links I) l)
              (inst_gran I) (inst_dflt I) (inst_root I) (inst_rootFeats I))
           (NPlus.CLink l).
     Proof.
       intros; apply T.VSet.ext; intro w.
       rewrite !versions_link_reduceReal; cbn [inst_repo inst_links inst_gran].
       rewrite crateReal_claimants,
-        linkRel_headFibre, <- ClsT.Reduction.Lookup.versions_lookupClass.
+        linkRel_withHead, <- ClsT.Reduction.Lookup.versions_lookupClass.
       reflexivity.
     Qed.
 
